---
title: Biology notes
tags:
  - mathematics
  - biology
  - chemistry
description: |
  Notes from studying organic chemistry
---

## Electron energy

### Frequency, wavelength and speed

$\nu$ is frequency

$\lambda$ is wavelength

$s$ is speed

#### Frequency

$$
\nu = \frac{s}{\lambda}
$$

#### Wavelength

$$
\lambda = \frac{s}{\nu}
$$

#### Speed

$$
s = \lambda\nu
$$

### For electromagnetic waves

$c$ is the speed of light ($3 \bullet 10^8\text{m}/\text{s}$ or, in $\text{nm}$ $3 \bullet 10^17\text{nm}/\text{s}$)

#### Frequency

$$
\nu = \frac{3 \bullet 10^17\text{nm}/\text{s}}{\lambda}
$$

If $\lambda$ is $w \bullet \text{nm}$

$$
\nu
$$

$$
= \frac{3 \bullet 10^17\frac{\text{nm}}{\text{s}}}{w \bullet \text{nm}}
$$

$$
= \frac{3 \bullet 10^17 \bullet \text{nm}\bullet \text{s}^(-1)}{w \bullet \text{nm}}
$$

$$
= 3 \bullet 10^17 \bullet \text{nm}\bullet \text{s}^(-1) \bullet (w \bullet \text{nm})^(-1)
$$

$$
= 3 \bullet 10^17 \bullet \text{nm}\bullet \text{s}^(-1) \bullet w^(-1) \bullet \text{nm}^(-1)
$$

$$
= 3 \bullet 10^17 \bullet \text{s}^(-1) \bullet w^(-1)
$$

$$
= 3 \bullet 10^17 \bullet (\text{s} \bullet w)^(-1)
$$

$$
= \frac{3 \bullet 10^17}{\text{s} \bullet w}
$$

$$
= \frac{3 \bullet 10^17}{w}/\text{s}
$$

#### Wavelength

$$
\lambda = \frac{3 \bullet 10^17\text{nm}/\text{s}}{\nu}
$$

If $\nu$ is $f/\text{s}$

$$
\lambda
$$

$$
= \frac{3 \bullet 10^17\frac{\text{nm}}{\text{s}}}{\frac{f}{\text{s}}}
$$

$$
= \frac{3 \bullet 10^17 \bullet \text{nm} \bullet \text{s}^(-1)}{f \bullet \text{s}^(-1)}
$$

$$
= 3 \bullet 10^17 \bullet \text{nm} \bullet \text{s}^(-1) \bullet (f \bullet \text{s}^(-1))^(-1)
$$

$$
= 3 \bullet 10^17 \bullet \text{nm} \bullet \text{s}^(-1) \bullet f^(-1) \bullet \text{s}^(-1)^(-1)
$$

$$
= 3 \bullet 10^17 \bullet \text{nm} \bullet \text{s}^(-1) \bullet f^(-1) \bullet \text{s}^(-1 \bullet -1)
$$

$$
= 3 \bullet 10^17 \bullet \text{nm} \bullet \text{s}^(-1) \bullet f^(-1) \bullet \text{s}
$$

$$
= 3 \bullet 10^17 \bullet \text{nm} \bullet f^(-1)
$$

$$
= \frac{3 \bullet 10^17}{f} \text{nm}
$$

### Photon energy

$$
E = h\nu
$$

Where $h$ is Planck's constant, $6.626 070 15 \times 10^(-34) \text{J} / \text{Hz}$ or $6.626 070 15 \times 10^(-34) \text{Js}$ owing to the fact that $\text{Hz} = 1/\text{s}$

Being that $\nu = \frac{c}{\lambda}$ we have:

$$
E
$$

$$
= h\nu
$$

$$
= h\frac{c}{\lambda}
$$

$$
= \frac{hc}{\lambda}
$$

$$
= \frac{h(3 \bullet 10^17\frac{\text{nm}}{\text{s}})}{\lambda}
$$

$$
= \frac{(6.626 070 15 \times 10^(-34)\text{Js})(3 \bullet 10^17\frac{\text{nm}}{\text{s}})}{\lambda}
$$

$$
= \frac{(6.626 070 15 \bullet 10^(-34) \bullet \text{J} \bullet \text{s})(3 \bullet 10^17 \bullet \text{nm} \bullet \text{s}^(-1))}{\lambda}
$$

$$
= \frac{6.626 070 15 \bullet 10^(-34) \bullet \text{J} \bullet \text{s} \bullet 3 \bullet 10^17 \bullet \text{nm} \bullet \text{s}^(-1)}{\lambda}
$$

$$
= \frac{6.626 070 15 \bullet 10^(-34) \bullet \text{J} \bullet 3 \bullet 10^17 \bullet \text{nm}}{\lambda}
$$

$$
= \frac{3 \bullet 6.626 070 15 \bullet 10^(-34) \bullet 10^17 \bullet \text{J} \bullet \text{nm}}{\lambda}
$$

$$
= \frac{3 \bullet 6.626 070 15 \bullet 10^(-17) \bullet \text{J} \bullet \text{nm}}{\lambda}
$$

$$
= \frac{19.87821045 \bullet 10^(-17) \bullet \text{J} \bullet \text{nm}}{\lambda}
$$

$$
= \frac{1.987821045 \bullet 10^(-16) \bullet \text{J} \bullet \text{nm}}{\lambda}
$$

Now suppose $\lambda$ is $w \bullet \text{nm}$

$$
= \frac{1.987821045 \bullet 10^(-16) \bullet \text{J} \bullet \text{nm}}{w \bullet \text{nm}}
$$

$$
= 1.987821045 \bullet 10^(-16) \bullet \text{J} \bullet \text{nm} \bullet (w \bullet \text{nm})^(-1)
$$

$$
= 1.987821045 \bullet 10^(-16) \bullet \text{J} \bullet \text{nm} \bullet w^(-1) \bullet \text{nm}^(-1)
$$

$$
= 1.987821045 \bullet 10^(-16) \bullet \text{J} \bullet w^(-1)
$$

$$
= 1.987821045 \bullet 10^(-16) \bullet w^(-1) \bullet \text{J}
$$

$$
= \frac{1.987821045 \times 10^(-16)}{w} \text{J}
$$

Alternatively, suppose $\lambda$ is $\frac{c}{\nu}$.

$$
= \frac{1.987821045 \bullet 10^(-16) \bullet \text{J} \bullet \text{nm}}{\frac{c}{\nu}}
$$

And $\nu$ is $f/\text{s}$.

$$
= \frac{1.987821045 \bullet 10^(-16) \bullet \text{J} \bullet \text{nm}}{\frac{c}{f/\text{s}}}
$$

Inline $c$.

$$
= \frac{1.987821045 \bullet 10^(-16) \bullet \text{J} \bullet \text{nm}}{\frac{3 \bullet 10^17\frac{\text{nm}}{\text{s}}}{f/\text{s}}}
$$

$$
= \frac{1.987821045 \bullet 10^(-16) \bullet \text{J} \bullet \text{nm}}{\frac{3 \bullet 10^17\frac{\text{nm}}{\text{s}}}{\frac{f}{\text{s}}}}
$$

$$
= \frac{1.987821045 \bullet 10^(-16) \bullet \text{J} \bullet \text{nm}}{\frac{3 \bullet 10^17\frac{\text{nm}}{\text{s}}}{f \bullet \text{s}^(-1)}}
$$

$$
= \frac{1.987821045 \bullet 10^(-16) \bullet \text{J} \bullet \text{nm}}{\frac{3 \bullet 10^17 \bullet \text{nm} \bullet \text{s}^(-1)}{f \bullet \text{s}^(-1)}}
$$

$$
= \frac{1.987821045 \bullet 10^(-16) \bullet \text{J} \bullet \text{nm}}{3 \bullet 10^17 \bullet \text{nm} \bullet \text{s}^(-1) \bullet (f \bullet \text{s}^(-1))^(-1)}
$$

$$
= 1.987821045 \bullet 10^(-16) \bullet \text{J} \bullet \text{nm} \bullet (3 \bullet 10^17 \bullet \text{nm} \bullet \text{s}^(-1) \bullet (f \bullet \text{s}^(-1))^(-1))^(-1)
$$

$$
= 1.987821045 \bullet 10^(-16) \bullet \text{J} \bullet \text{nm} \bullet (3 \bullet 10^17 \bullet \text{nm} \bullet \text{s}^(-1) \bullet f^(-1) \bullet \text{s}^(-1 \bullet -1))^(-1)
$$

$$
= 1.987821045 \bullet 10^(-16) \bullet \text{J} \bullet \text{nm} \bullet 3^(-1) \bullet 10^17^(-1) \bullet \text{nm}^(-1) \bullet \text{s}^(-1)^(-1) \bullet f^(-1)^(-1) \bullet \text{s}^(-1 \bullet -1)^(-1)
$$

$$
= 1.987821045 \bullet 10^(-16) \bullet \text{J} \bullet \text{nm} \bullet 3^(-1) \bullet 10^(17 \bullet -1) \bullet \text{nm}^(-1) \bullet \text{s}^(-1 \bullet -1) \bullet f^(-1 \bullet -1) \bullet \text{s}^(-1 \bullet -1 \bullet -1)
$$

$$
= 1.987821045 \bullet 10^(-16) \bullet \text{J} \bullet \text{nm} \bullet 3^(-1) \bullet 10^(-17) \bullet \text{nm}^(-1) \bullet \text{s} \bullet f \bullet \text{s}^(-1)
$$

$$
= 1.987821045 \bullet 3^(-1) \bullet 10^(-16) \bullet 10^(-17) \bullet \text{J} \bullet \text{nm} \bullet \text{nm}^(-1) \bullet \text{s} \bullet \text{s}^(-1) \bullet f
$$

$$
= 1.987821045 \bullet 3^(-1) \bullet 10^(-16 - 17) \bullet \text{J} \bullet f
$$

$$
= 1.987821045 \bullet 3^(-1) \bullet 10^(-33) \bullet \text{J} \bullet f
$$

$$
= 0.662607015f \times 10^(-33) \text{J}
$$

$$
= 6.62607015f \times 10^(-34) \text{J}
$$

### Hydrogen electron energy

$$
E_n = -R_H(\frac{1}{n^2})
$$

$n$ is the principal quantum number. The electron shell, $1, 2, 3 ...$. Electrons in different orbitals with the same principal atomic number have the same energy. Shape ($l$) or orientation ($m_l$) have no effect on energy.

$R_H$ is the Rydberg constant, $2.18 \times 10^(-18)\text{J}$

$$
E_n
$$

$$
= -R_H(\frac{1}{n^2})
$$

$$
= -2.18 \bullet 10^(-18) \bullet \text{J} \bullet n^2^(-1)
$$

$$
= -2.18 \bullet 10^(-18) \bullet n^2^(-1) \bullet \text{J}
$$

$$
= \frac{-2.18 \bullet 10^(-18)}{n^2} \text{J}
$$

### Hydrogen photon emission energy

When electrons "descend" from a higher energy shell to a lower energy shell they emit a photon. The following equation gives the energy difference of the two shells. The compliment of this then should be the energy of the emitted photon. The energy lost is equal to the energy emitted as a photon.

$$
\Delta E = E_j - E_i
$$

Where $E_j$ is the energy of shell the electron has moved _to_ and $E_i$ is the energy of the shell the electron has moved _from_.

$$
\Delta E = E_j - E_i
$$

$$
\Delta E
$$

$$
= E_j - E_i
$$

$$
= -R_H(\frac{1}{n_j^2}) - (-R_H(\frac{1}{n_i^2}))
$$

$$
= -1 \bullet R_H(\frac{1}{n_j^2}) + -1 \bullet (-1 \bullet R_H(\frac{1}{n_i^2}))
$$

$$
= -1 \bullet R_H \bullet n_j^2^(-1) + -1 \bullet -1 \bullet R_H \bullet n_i^2^(-1)
$$

$$
= -1 \bullet R_H \bullet n_j^2^(-1) + R_H \bullet n_i^2^(-1)
$$

$$
= R_H \bullet n_i^2^(-1) + -1 \bullet R_H \bullet n_j^2^(-1)
$$

$$
= R_H \bullet n_i^2^(-1) + R_H \bullet -1 \bullet n_j^2^(-1)
$$

$$
= R_H \bullet (n_i^2^(-1) + -1 \bullet n_j^2^(-1))
$$

$$
= R_H (\frac{1}{n_i^2} - \frac{1}{n_j^2})
$$

Or, with the Rydberg constant inlined:

$$
= (2.18 \times 10^(-18)) (\frac{1}{n_i^2} - \frac{1}{n_j^2}) \text{J}
$$

For example if moving from the 4 shell to the 2 shell we have.

$$
= (2.18 \times 10^(-18)) (\frac{1}{4^2} - \frac{1}{2^2}) \text{J}
$$

$$
= (2.18 \times 10^(-18)) (\frac{1}{16} - \frac{1}{4}) \text{J}
$$

$$
= (2.18 \times 10^(-18)) (\frac{1}{16} + \frac{-1}{4}) \text{J}
$$

$$
= (2.18 \times 10^(-18)) (\frac{1 \bullet 4 + -1 \bullet 16}{16 \bullet 4}) \text{J}
$$

$$
= (2.18 \times 10^(-18)) (\frac{-12}{64}) \text{J}
$$

$$
= (2.18 \times 10^(-18)) (\frac{-3}{16}) \text{J}
$$

$$
= 2.18 \bullet 10^(-18) \bullet -3 \bullet 16^(-1) \bullet \text{J}
$$

$$
= 2.18 \bullet -3 \bullet 16^(-1) \bullet 10^(-18) \bullet \text{J}
$$

$$
= −0.40875 \times 10^(-18) \text{J}
$$

$$
= −4.0875 \times 10^(-19) \text{J}
$$

Suffice it to say: a very small amount of energy.

## Solute potential

$$
ψ_s = -i\text{CRT}
$$

$i$ is the ionisation constant (unitless)

$\text{C}$ is the molar concentration ($c\text{M}$  or $c\frac{\text{mol}}{\text{L}}$)

$\text{R}$ is the pressure constant ($0.0831 \frac{\text{L} \bullet \text{bar}}{(\text{mol} \bullet \text{K})}$)

$\text{T}$ is the temperature in Kelvin ($t\text{K}$)

$$
\psi_s
$$

$$
= -i\text{CRT}
$$


$$
= -i(c\frac{\text{mol}}{\text{L}})(0.0831 \frac{\text{L} \bullet \text{bar}}{(\text{mol} \bullet \text{K})})(t\text{K})
$$

$$
= -i(c \bullet \text{mol} \bullet \text{L}^(-1))(0.0831 \text{L} \bullet \text{bar} \bullet \text{mol}^(-1) \bullet \text{K}^(-1))(t \bullet \text{K})
$$

$$
= -i \bullet c \bullet \text{mol} \bullet \text{L}^(-1) \bullet 0.0831 \bullet \text{L} \bullet \text{bar} \bullet \text{mol}^(-1) \bullet \text{K}^(-1) \bullet t \bullet \text{K}
$$

$$
= 0.0831 \bullet -i \bullet c \bullet t \bullet \text{bar} \bullet \text{mol} \bullet \text{mol}^(-1) \bullet \text{L} \bullet \text{L}^(-1) \bullet \text{K} \bullet \text{K}^(-1)
$$

$$
= 0.0831 \bullet -i \bullet c \bullet t \bullet \text{bar}
$$

$$
= -(0.0831ict) \text{bar}
$$
